examples/Crypto/DES/des_propScript.sml
@@ -1608,30 +1608,6 @@ Proof
   >> rw[extreal_mul_eq]
 QED
 
-Theorem XcauseYFp_eq:   
-   !X Y. Xe=E(X) /\ x1=(5><0) Xe /\ x2=(11><6) Xe /\x3=(17><12) Xe /\x4=(23><18) Xe /\x5=(29><24) Xe /\x6=(35><30) Xe /\x7=(41><36) Xe /\x8=(47><42) Xe /\y1=(3><0) Y /\y2=(7><4) Y /\y3=(11><8) Y /\y4=(15><12) Y /\y5=(19><16) Y /\y6=(23><20) Y /\y7=(27><24) Y /\y8=(31><28) Y ==>
-   XcauseYF' X Y = (XcauseY x8 y8 S1)*(XcauseY x7 y7 S2)*(XcauseY x6 y6 S3)*(XcauseY x5 y5 S4)*(XcauseY x4 y4 S5)*(XcauseY x3 y3 S6)*(XcauseY x2 y2 S7)*(XcauseY x1 y1 S8)
-Proof
-     rw[XcauseYF'_def,XcauseY_def]
-  >> rw[word6p_def,word48p_def]
-  >> rw[prob_def]
-  >> rw[CARD_eqF]
-  >> rw[F_convert]
-  >> rw[CARD_CROSS]
-  >> Q.ABBREV_TAC ‘n1=CARD {x | S1 x ⊕ S1 (x ⊕ (47 >< 42) (E X)) = (31 >< 28) Y}’
-  >> Q.ABBREV_TAC ‘n2=CARD {x | S2 x ⊕ S2 (x ⊕ (41 >< 36) (E X)) = (27 >< 24) Y}’
-  >> Q.ABBREV_TAC ‘n3=CARD {x | S3 x ⊕ S3 (x ⊕ (35 >< 30) (E X)) = (23 >< 20) Y} ’
-  >>  Q.ABBREV_TAC ‘n4=CARD {x | S4 x ⊕ S4 (x ⊕ (29 >< 24) (E X)) = (19 >< 16) Y}’
-  >>  Q.ABBREV_TAC ‘n5=CARD {x | S5 x ⊕ S5 (x ⊕ (23 >< 18) (E X)) = (15 >< 12) Y}’
-  >>  Q.ABBREV_TAC ‘n6=CARD {x | S6 x ⊕ S6 (x ⊕ (17 >< 12) (E X)) = (11 >< 8) Y}’
-  >> Q.ABBREV_TAC ‘n7= CARD {x | S7 x ⊕ S7 (x ⊕ (11 >< 6) (E X)) = (7 >< 4) Y}’
-  >> Q.ABBREV_TAC ‘n8=CARD {x | S8 x ⊕ S8 (x ⊕ (5 >< 0) (E X)) = (3 >< 0) Y}’
-  >> rw[extreal_of_num_def]
-  >> rw[div_eq_mul_linv]
-  >> rw[extreal_inv_eq]
-  >> rw[extreal_mul_eq]
-QED
-
 Definition transktoxF_def:
   transktoxF (x:word48) k= k ?? x
 End
